split CreateWrite into separate Create and Write

src/Mail/MailFSImpl.v
@@ -24,6 +24,10 @@ Module MailFSImpl' <:
     l <- Call (MailFSOp.List);
     Ret (map snd (filter (same_tid tid) l)).
 
+  Definition createwrite_core data :=
+    ok1 <- Call (MailFSOp.CreateTmp);
+    if (ok1 : bool) then Call (MailFSOp.WriteTmp data) else Ret ok1.
+
   Definition compile_op T (op : DeliverListTidOp.Op T) : proc _ T :=
     match op with
     | DeliverListTidOp.LinkMail m => Call (MailFSOp.LinkMail m)
@@ -31,7 +35,7 @@ Module MailFSImpl' <:
     | DeliverListTidOp.ListTid => listtid_core
     | DeliverListTidOp.Read fn => Call (MailFSOp.Read fn)
     | DeliverListTidOp.Delete fn => Call (MailFSOp.Delete fn)
-    | DeliverListTidOp.CreateWriteTmp data => Call (MailFSOp.CreateWriteTmp data)
+    | DeliverListTidOp.CreateWriteTmp data => createwrite_core data
     | DeliverListTidOp.UnlinkTmp => Call (MailFSOp.UnlinkTmp)
     | DeliverListTidOp.Lock => Call (MailFSOp.Lock)
     | DeliverListTidOp.Unlock => Call (MailFSOp.Unlock)
@@ -45,6 +49,9 @@ Module MailFSImpl' <:
       no_atomics (compile_op op).
   Proof.
     destruct op; compute; eauto.
+
+    constructor; eauto.
+    destruct x; eauto.
   Qed.
 
   Ltac step_inv :=
@@ -59,6 +66,7 @@ Module MailFSImpl' <:
 
   Hint Extern 1 (MailFSAPI.step _ _ _ _ _ _) => econstructor.
   Hint Extern 1 (DeliverListTidAPI.step _ _ _ _ _ _) => econstructor.
+  Hint Constructors MailFSAPI.xstep.
 
   Lemma gettid_right_mover :
     right_mover
@@ -68,10 +76,48 @@ Module MailFSImpl' <:
     unfold right_mover; intros.
     repeat step_inv; eauto 10.
 
-    eexists; split; econstructor.
+    eexists; split; econstructor; eauto.
   Qed.
 
   Hint Resolve gettid_right_mover.
+
+  Lemma fmap_in_tid_ne :
+    forall (tid0 tid1 : nat) (x y : nat) TV (v : TV) m,
+      tid0 <> tid1 ->
+      FMap.In (tid0, x) (FMap.add (tid1, y) v m) ->
+      FMap.In (tid0, x) m.
+  Proof.
+    intros.
+    eapply FMap.in_add_ne; eauto.
+    congruence.
+  Qed.
+
+  Hint Resolve fmap_in_tid_ne.
+
+  Lemma createtmp_right_mover :
+    right_mover
+      MailFSAPI.step
+      (MailFSOp.CreateTmp).
+  Proof.
+    unfold right_mover; intros.
+    repeat step_inv; eauto 10.
+
+    all: unfold MailFSAPI.step.
+    all: try solve [ rewrite FMap.add_add_ne by congruence; eauto 10 ].
+
+    rewrite FMap.add_add_ne by congruence.
+      eexists. split. 2: eauto. eauto.
+
+    rewrite <- FMap.add_remove_ne by congruence.
+      eexists. split. 2: eauto. eauto.
+
+    eapply FMap.mapsto_add_ne in H12; try congruence.
+      eexists. split. 2: eauto. eauto.
+
+    eexists. split. 2: eauto. eauto.
+  Qed.
+
+  Hint Resolve createtmp_right_mover.
 
   Theorem ysa_movers_listtid_core:
     ysa_movers MailFSAPI.step listtid_core.
@@ -80,6 +126,16 @@ Module MailFSImpl' <:
   Qed.
 
   Hint Resolve ysa_movers_listtid_core.
+
+  Theorem ysa_movers_createwrite_core:
+    forall data,
+      ysa_movers MailFSAPI.step (createwrite_core data).
+  Proof.
+    econstructor; eauto 20.
+    destruct r; eauto 20.
+  Qed.
+
+  Hint Resolve ysa_movers_createwrite_core.
 
   Theorem ysa_movers : forall `(op : _ T),
     ysa_movers MailFSAPI.step (compile_op op).
@@ -95,16 +151,20 @@ Module MailFSImpl' <:
 
     all: try solve [ repeat atomic_exec_inv; repeat step_inv; eauto ].
 
-    repeat atomic_exec_inv.
-    repeat step_inv; eauto.
-    econstructor; intros.
+    - repeat atomic_exec_inv; repeat step_inv; eauto.
+      rewrite FMap.add_add; eauto.
+      rewrite FMap.add_add; eauto.
 
-    eapply in_map_iff.
-    exists (v1, fn); intuition eauto.
-    eapply filter_In; intuition eauto.
-    eapply FMap.is_permutation_in'; eauto.
-    unfold same_tid; simpl.
-    destruct (v1 == v1); congruence.
+    - repeat atomic_exec_inv.
+      repeat step_inv; eauto.
+      econstructor; intros.
+
+      eapply in_map_iff.
+      exists (v1, fn); intuition eauto.
+      eapply filter_In; intuition eauto.
+      eapply FMap.is_permutation_in'; eauto.
+      unfold same_tid; simpl.
+      destruct (v1 == v1); congruence.
   Qed.
 
   Definition initP_compat : forall s, MailFSAPI.initP s ->
